Refactoring insertion circuit

formal-verification/FormalVerification/SemanticEquivalence/Insertion.lean
@@ -19,15 +19,18 @@ open SemaphoreMTB renaming InsertionProof_4_30_4_4_30 → gInsertionProof
 
 -- Insertion round semantic equivalence
 
-def insertion_round (Index: F) (Item: F) (PrevRoot: F) (Proof: Vector F D) (k: F -> Prop) : Prop :=
+def insertion_round (Path: Vector F D) (Item: F) (PrevRoot: F) (Proof: Vector F D) (k: F -> Prop) : Prop :=
+  (MerkleTree.recover_tail poseidon₂ (Dir.create_dir_vec Path) Proof 0 = PrevRoot) ∧
+  k (MerkleTree.recover_tail poseidon₂ (Dir.create_dir_vec Path) Proof Item)
+
+def insertion_round_prep (Index: F) (Item: F) (PrevRoot: F) (Proof: Vector F D) (k: F -> Prop) : Prop :=
   ∃out: Vector F D, recover_binary_zmod' out = Index ∧ is_vector_binary out ∧
-  (MerkleTree.recover_tail poseidon₂ (Dir.create_dir_vec out) Proof 0 = PrevRoot) ∧
-  k (MerkleTree.recover_tail poseidon₂ (Dir.create_dir_vec out) Proof Item)
+  insertion_round out Item PrevRoot Proof k
 
 lemma InsertionRound_uncps {Index: F} {Item: F} {PrevRoot: F} {Proof: Vector F D} {k: F -> Prop} :
   gInsertionRound Index Item PrevRoot Proof k ↔
-  insertion_round Index Item PrevRoot Proof k := by
-  simp [insertion_round]
+  insertion_round_prep Index Item PrevRoot Proof k := by
+  simp [insertion_round_prep, insertion_round]
   simp [gInsertionRound]
   simp [Gates.to_binary, Gates.eq]
   simp [VerifyProof_looped, proof_rounds_uncps]
@@ -50,9 +53,8 @@ def InsertionLoop {n} (StartIndex: F) (PreRoot: F) (IdComms: Vector F n) (Merkle
   match n with
   | Nat.zero => k PreRoot
   | Nat.succ _ =>
-    ∃out: Vector F D, recover_binary_zmod' out = StartIndex ∧ is_vector_binary out ∧
-    MerkleTree.recover_tail poseidon₂ (Dir.create_dir_vec out) MerkleProofs.head 0 = PreRoot ∧
-    InsertionLoop (StartIndex + 1) (MerkleTree.recover_tail poseidon₂ (Dir.create_dir_vec out) MerkleProofs.head IdComms.head) IdComms.tail MerkleProofs.tail k
+    insertion_round_prep StartIndex IdComms.head PreRoot MerkleProofs.head fun next =>
+    InsertionLoop (StartIndex + 1) next IdComms.tail MerkleProofs.tail k
 
 lemma insertion_rounds_uncps {n} {StartIndex: F} {PreRoot: F} {IdComms: Vector F n} {MerkleProofs: Vector (Vector F D) n} {k : F -> Prop}:
   insertion_rounds StartIndex PreRoot IdComms MerkleProofs k ↔
@@ -65,7 +67,7 @@ lemma insertion_rounds_uncps {n} {StartIndex: F} {PreRoot: F} {IdComms: Vector F
   | cons =>
     unfold insertion_rounds
     unfold InsertionLoop
-    simp [InsertionRound_uncps, insertion_round]
+    simp [InsertionRound_uncps, insertion_round_prep, insertion_round]
     rename_i ih
     simp [ih]
 
